Lemma Definition Checkpoint

Exp_lemmas.v
@@ -6,6 +6,7 @@ Require Export Metalib.Metatheory.
 Require Export Metalib.LibLNgen.
 
 From Exp Require Export Exp_ott.
+From Exp Require Export Exp_inf.
 
 (*************************************************************************)
 (** Notation, manually added *)
@@ -38,7 +39,7 @@ Notation "f x .. y" := (.. (f x) .. y)
 
 
 Notation "x" := x (in custom exp at level 0, x constr at level 0) : exp_scope.
-(* Notation "S -> T" := (Ty_Arrow S T) (in custom exp at level 50, right associativity) : exp_scope *)
+(* Notation "S -> T" := (ty_mono_func S T) (in custom exp at level 50, right associativity) : exp_scope *)
 Notation "x y" := (exp_app x y) (in custom exp at level 1, left associativity) : exp_scope.
 Notation "\ x : t , y" :=
   (exp_abs x t y) (in custom exp at level 90, x at level 99,
@@ -47,24 +48,6 @@ Notation "\ x : t , y" :=
                      left associativity) : exp_scope.
 
 Local Open Scope exp_scope.                     
-
-(* Variant of is_value_of_tm which is type Prop instead of bool *)
-Definition is_value (t : tm) : Prop := 
-  match t with 
-  | exp_lit _ => True 
-  | exp_abs _ => True 
-  | exp_typed_abs _ _ => True 
-  | _ => False 
-  end.
-
-
-(* Inductive value : tm -> Prop :=
-  | v_int : forall (i : integer), 
-      value <{ exp_lit i }>
-  | v_abs : forall x T2 t1,
-      value <{ \ x : T2 , t1 }>.
-       *)
-
 
 
 
@@ -81,18 +64,47 @@ Proof.
   intros t HT HVal.
   destruct HVal. *)
 
+Theorem unique_typing: forall t T1 T2,
+  typing empty t (ty_poly_rho T1)
+    -> typing empty t (ty_poly_rho T2)
+    -> T1 = T2.
+Proof with eauto.
+  intros t. induction t; intros.
+  - inversion H; inversion H0; subst...
+    + inversion H7.
+    + 
+Admitted.
 
+Theorem canonical_forms_fun: forall G t T1 T2,
+  typing G t (ty_poly_rho (ty_rho_tau (ty_mono_func T1 T2)))
+    -> is_value_of_tm t 
+    -> exists u, t = exp_abs u.
+Proof with eauto.
+  intros. induction t...
+  - (* exp_lit i = exp_abs u *)
+    induction H...
+  
+Admitted.
 
 
 Theorem progress : forall e T,
   typing empty e T ->
-  is_value e \/ exists e', step e e'.
-Proof.
+  is_value_of_tm e \/ exists e', step e e'.
+Proof with eauto.
   intros e T H.
-  assert (typing empty e T); auto.
-  induction H; subst; auto.
-  - (* exp_lit *)
-   left. admit.
-  - (* exp_lit duplicate *)
-    admit.
-  Admitted.
+  (* We induct on the term e so that we always have a hypothesis 
+    involving the empty context. *)
+  induction e; subst; auto;
+  try (left; constructor).
+  - (* var shouldn't have a type in the empty context *)
+    inversion H; subst...
+    
+Admitted.
+
+
+Theorem preservation : forall (E : ctx) e e' T,
+  typing E e T
+    -> step e e'
+    -> typing E e' T.
+Proof.
+  intros E e e' T Htyp Hstep. 
