Exp_thm.v
@@ -1,3 +1,0 @@
-From Exp Require Export Exp_ott.
-
-
